src/simulation/Cert_ar.v
@@ -1,0 +1,889 @@
+From hahn Require Import Hahn.
+
+From imm Require Import Events.
+From imm Require Import Execution.
+From imm Require Import Execution_eco.
+From imm Require Import imm_bob imm_s_ppo.
+From imm Require Import imm_s_hb.
+From imm Require Import imm_s.
+From imm Require Import imm_common_more.
+From imm Require Import CertCOhelper.
+From imm Require Import CombRelations.
+
+Require Import AuxRel2.
+Require Import TraversalConfig.
+Require Import TraversalConfigAlt.
+Require Import TraversalConfigAltOld.
+Require Import ExtTraversalConfig.
+
+Require Import ImmProperties.
+
+Require Import Cert_co.
+Require Import Cert_D.
+Require Import Cert_rf.
+Require Import CertExecution2.
+
+Set Implicit Arguments.
+Remove Hints plus_n_O.
+
+Notation "'Tid_' t" := (fun x => tid x = t) (at level 1).
+Notation "'NTid_' t" := (fun x => tid x <> t) (at level 1).
+
+Section CertExec_ar.
+
+Variable G : execution.
+Variable sc : relation actid.
+
+Notation "'Init'" := (fun a => is_true (is_init a)).
+
+Notation "'E'" := G.(acts_set).
+Notation "'Gacts'" := G.(acts).
+Notation "'Glab'" := G.(lab).
+Notation "'Gsb'" := G.(sb).
+Notation "'Grf'" := G.(rf).
+Notation "'Gco'" := G.(co).
+Notation "'Grmw'" := G.(rmw).
+Notation "'Gdata'" := G.(data).
+Notation "'Gaddr'" := G.(addr).
+Notation "'Gctrl'" := G.(ctrl).
+Notation "'Gdeps'" := G.(deps).
+Notation "'Grmw_dep'" := G.(rmw_dep).
+
+Notation "'Gfre'" := G.(fre).
+Notation "'Grfe'" := G.(rfe).
+Notation "'Gcoe'" := G.(coe).
+Notation "'Grfi'" := G.(rfi).
+Notation "'Gfri'" := G.(fri).
+Notation "'Gcoi'" := G.(coi).
+Notation "'Gfr'" := G.(fr).
+Notation "'Geco'" := G.(eco).
+Notation "'Gdetour'" := G.(detour).
+Notation "'Gsw'" := G.(sw).
+Notation "'Grelease'" := G.(release).
+Notation "'Grs'" := G.(rs).
+Notation "'Ghb'" := G.(hb).
+Notation "'Gppo'" := G.(ppo).
+Notation "'Grppo'" := G.(rppo).
+Notation "'Gbob'" := G.(bob).
+Notation "'Gfwbob'" := G.(fwbob).
+Notation "'Gar'" := (G.(ar) sc).
+Notation "'Gar_int'" := (G.(ar_int)).
+Notation "'Gurr'" := (G.(urr) sc).
+Notation "'Gfurr'" := (G.(furr) sc).
+Notation "'Gmsg_rel'" := (G.(msg_rel) sc).
+
+Notation "'Gloc'" := (loc Glab).
+Notation "'Gval'" := (val Glab).
+Notation "'Gsame_loc'" := (same_loc Glab).
+
+Notation "'R'" := (fun a => is_true (is_r Glab a)).
+Notation "'W'" := (fun a => is_true (is_w Glab a)).
+Notation "'F'" := (fun a => is_true (is_f Glab a)).
+Notation "'GR_ex'" := (fun a => is_true (R_ex Glab a)).
+Notation "'GW_ex'" := G.(W_ex).
+Notation "'GW_ex_acq'" := (GW_ex ∩₁ (fun a => is_true (is_xacq Glab a))).
+
+Notation "'Loc_' l" := (fun x => Gloc x = Some l) (at level 1).
+Notation "'W_' l" := (W ∩₁ Loc_ l) (at level 1).
+Notation "'R_' l" := (R ∩₁ Loc_ l) (at level 1).
+
+Notation "'Pln'" := (fun a => is_true (is_only_pln Glab a)).
+Notation "'Rlx'" := (fun a => is_true (is_rlx Glab a)).
+Notation "'Rel'" := (fun a => is_true (is_rel Glab a)).
+Notation "'Acq'" := (fun a => is_true (is_acq Glab a)).
+Notation "'Acqrel'" := (fun a => is_true (is_acqrel Glab a)).
+Notation "'Acq/Rel'" := (fun a => is_true (is_ra Glab a)).
+Notation "'Sc'" := (fun a => is_true (is_sc Glab a)).
+Notation "'xacq'" := (fun a => is_true (is_xacq Glab a)).
+
+
+Variable T : trav_config.
+Variable S : actid -> Prop.
+
+Notation "'I'" := (issued T).
+Notation "'C'" := (covered T).
+
+Variable thread : BinNums.positive.
+
+Notation "'cert_co'" := (cert_co G T thread).
+
+Notation "'D'" := (D G T S thread).
+
+Notation "'new_rf'" := (new_rf G sc T S thread).
+Notation "'cert_rf'" := (cert_rf G sc T S thread).
+Notation "'cert_rfi'" := (cert_rfi G sc T S thread).
+Notation "'cert_rfe'" := (cert_rfe G sc T S thread).
+
+Hypothesis WF : Wf G.
+Hypothesis WF_SC : wf_sc G sc.
+Hypothesis RELCOV : W ∩₁ Rel ∩₁ I ⊆₁ C.
+Hypothesis TCCOH : tc_coherent G sc T.
+Hypothesis ACYC_EXT : acyc_ext G sc.
+Hypothesis CSC : coh_sc G sc.
+Hypothesis COH : coherence G.
+Hypothesis AT : rmw_atomicity G.
+
+Hypothesis IT_new_co: I ∪₁ E ∩₁ W ∩₁ Tid_ thread ≡₁ E ∩₁ W.
+Hypothesis E_to_S: E ⊆₁ C ∪₁ dom_rel (Gsb^? ⨾ ⦗S⦘).
+Hypothesis Grfe_E : dom_rel Grfe ⊆₁ I.
+Hypothesis E_F_AcqRel_in_C: E ∩₁ F ∩₁ Acq/Rel ⊆₁ C.
+Hypothesis COMP_ACQ: forall r (IN: (E ∩₁ R ∩₁ Acq) r), exists w, Grf w r.
+Hypothesis urr_helper: dom_rel ((Ghb ⨾ ⦗F ∩₁ Sc⦘)^? ⨾ sc^? ⨾ Ghb^? ⨾ Grelease ⨾ ⦗I⦘) ⊆₁ C.
+Hypothesis urr_helper_C: dom_rel ((Ghb ⨾ ⦗F ∩₁ Sc⦘)^? ⨾ sc^? ⨾ Ghb^? ⨾ (Grelease ⨾ Grf)^? ⨾ ⦗C⦘) ⊆₁ C.
+Hypothesis W_hb_sc_hb_to_I_NTid: dom_rel (⦗W⦘ ⨾ Ghb ⨾ (sc ⨾ Ghb)^? ⨾ ⦗I ∩₁ NTid_ thread⦘) ⊆₁ I.
+Hypothesis detour_E : dom_rel (Gdetour ⨾ ⦗E ∩₁ NTid_ thread⦘) ⊆₁ I.
+Hypothesis detour_Acq_E : dom_rel (Gdetour ⨾ ⦗E ∩₁ R ∩₁ Acq⦘) ⊆₁ I.
+Hypothesis hb_sc_hb_de : ⦗(E \₁ C) ∩₁ (E \₁ I)⦘ ⨾ Ghb ⨾ (sc ⨾ Ghb)^? ⊆ Gsb.
+Hypothesis COMP_C : C ∩₁ R ⊆₁ codom_rel Grf.
+Hypothesis COMP_NTID : E ∩₁ NTid_ thread ∩₁ R ⊆₁ codom_rel Grf.
+Hypothesis COMP_PPO : dom_rel (Gppo ⨾ ⦗I⦘) ⊆₁ codom_rel Grf.
+Hypothesis COMP_RPPO : dom_rel (⦗R⦘ ⨾ (Gdata ∪ Grfi ∪ Grmw)＊ ⨾ Grppo ⨾ ⦗S⦘) ⊆₁ codom_rel Grf.
+Hypothesis TCCOH_rst_new_T : tc_coherent G sc (mkTC (C ∪₁ (E ∩₁ NTid_ thread)) I).
+
+Hypothesis S_in_W : S ⊆₁ W.
+Hypothesis RPPO_S : dom_rel ((Gdetour ∪ Grfe) ⨾ (Gdata ∪ Grfi ∪ Grmw)＊ ⨾ Grppo ⨾ ⦗S⦘) ⊆₁ I.
+Hypothesis ST_in_E : S ∩₁ Tid_ thread ⊆₁ E.
+Hypothesis I_in_S : I ⊆₁ S.
+Hypothesis W_ex_acq_in_I :GW_ex_acq ⊆₁ I.
+
+Hypothesis F_in_C : E ∩₁ F ∩₁ Acq/Rel ⊆₁ C.
+
+Hypothesis S_I_in_W_ex : (S ∩₁ Tid_ thread) \₁ I ⊆₁ W_ex G.
+
+Hypothesis ETC_DR_R_ACQ_I : dom_rel ((Gdetour ∪ Grfe) ⨾ (Grmw ⨾ Grfi)^* ⨾ ⦗R∩₁Acq⦘ ⨾ Gsb ⨾ ⦗S⦘) ⊆₁ I.
+
+Hypothesis COMP_R_ACQ_SB : dom_rel ((Grmw ⨾ Grfi)＊ ⨾ ⦗E ∩₁ R ∩₁ Acq⦘) ⊆₁ codom_rel Grf.
+
+Variable lab' : actid -> label.
+Hypothesis SAME : same_lab_u2v lab' Glab.
+
+Notation "'certG'" := (certG G sc T S thread lab').
+
+
+(* Notation "'CE'" := certG.(acts_set). *)
+(* Notation "'Cacts'" := certG.(acts). *)
+(* Notation "'Clab'" := certG.(lab). *)
+(* Notation "'Csb'" := certG.(sb). *)
+Notation "'Crf'" := certG.(rf).
+Notation "'Cco'" := certG.(co).
+Notation "'Crmw'" := certG.(rmw).
+(* Notation "'Cdata'" := certG.(data). *)
+(* Notation "'Caddr'" := certG.(addr). *)
+(* Notation "'Cctrl'" := certG.(ctrl). *)
+Notation "'Cdeps'" := certG.(deps).
+(* Notation "'Crmw_dep'" := certG.(rmw_dep). *)
+
+Notation "'Cfre'" := certG.(fre).
+(* Notation "'Crfe'" := certG.(rfe). *)
+Notation "'Ccoe'" := certG.(coe).
+Notation "'Crfi'" := certG.(rfi).
+Notation "'Cfri'" := certG.(fri).
+Notation "'Ccoi'" := certG.(coi).
+Notation "'Cfr'" := certG.(fr).
+Notation "'Ceco'" := certG.(eco).
+Notation "'Cdetour'" := certG.(detour).
+Notation "'Csw'" := certG.(sw).
+Notation "'Crelease'" := certG.(release).
+Notation "'Crs'" := certG.(rs).
+Notation "'Chb'" := certG.(hb).
+Notation "'Cppo'" := certG.(ppo).
+(* Notation "'Cbob'" := certG.(bob). *)
+(* Notation "'Cfwbob'" := certG.(fwbob). *)
+Notation "'Car'" := (certG.(ar) sc).
+Notation "'Car_int'" := (certG.(ar_int)).
+Notation "'Curr'" := (certG.(urr) sc).
+Notation "'Cmsg_rel'" := (certG.(msg_rel) sc).
+
+(* Notation "'E'" := G.(acts_set). *)
+(* Notation "'Gacts'" := G.(acts). *)
+Notation "'Clab'" := certG.(lab).
+Notation "'Csb'" := certG.(sb).
+(* Notation "'Grf'" := G.(rf). *)
+(* Notation "'Gco'" := G.(co). *)
+(* Notation "'Gdata'" := G.(data). *)
+(* Notation "'Gaddr'" := G.(addr). *)
+(* Notation "'Gctrl'" := G.(ctrl). *)
+(* Notation "'Gdeps'" := G.(deps). *)
+(* Notation "'Grmw_dep'" := G.(rmw_dep). *)
+
+(* Notation "'Gfre'" := G.(fre). *)
+Notation "'Crfe'" := certG.(rfe).
+(* Notation "'Gcoe'" := G.(coe). *)
+Notation "'Crfi'" := certG.(rfi).
+(* Notation "'Gfri'" := G.(fri). *)
+(* Notation "'Gcoi'" := G.(coi). *)
+(* Notation "'Gfr'" := G.(fr). *)
+(* Notation "'Geco'" := G.(eco). *)
+(* Notation "'Gdetour'" := G.(detour). *)
+(* Notation "'Gsw'" := G.(sw). *)
+Notation "'Crelease'" := certG.(release).
+(* Notation "'Grs'" := G.(rs). *)
+(* Notation "'Ghb'" := G.(hb). *)
+(* Notation "'Gppo'" := G.(ppo). *)
+(* Notation "'Grppo'" := G.(rppo). *)
+(* Notation "'Gbob'" := G.(bob). *)
+(* Notation "'Gfwbob'" := G.(fwbob). *)
+(* Notation "'Gar'" := (G.(ar) sc). *)
+(* Notation "'Gar_int'" := (G.(ar_int)). *)
+(* Notation "'Gurr'" := (G.(urr) sc). *)
+(* Notation "'Gfurr'" := (G.(furr) sc). *)
+(* Notation "'Gmsg_rel'" := (G.(msg_rel) sc). *)
+
+(* Notation "'Gloc'" := (loc Glab). *)
+(* Notation "'Gval'" := (val Glab). *)
+Notation "'Csame_loc'" := (same_loc Clab).
+
+Notation "'CR'" := (fun a => is_true (is_r Clab a)).
+Notation "'CW'" := (fun a => is_true (is_w Clab a)).
+Notation "'CF'" := (fun a => is_true (is_f Clab a)).
+(* Notation "'GR_ex'" := (fun a => is_true (R_ex Glab a)). *)
+(* Notation "'GW_ex'" := G.(W_ex). *)
+(* Notation "'GW_ex_acq'" := (GW_ex ∩₁ (fun a => is_true (is_xacq Glab a))). *)
+
+Notation "'CPln'" := (fun a => is_true (is_only_pln Clab a)).
+Notation "'CRlx'" := (fun a => is_true (is_rlx Clab a)).
+Notation "'CRel'" := (fun a => is_true (is_rel Clab a)).
+Notation "'CAcq'" := (fun a => is_true (is_acq Clab a)).
+Notation "'CAcqrel'" := (fun a => is_true (is_acqrel Clab a)).
+Notation "'CAcq/Rel'" := (fun a => is_true (is_ra Clab a)).
+Notation "'CSc'" := (fun a => is_true (is_sc Clab a)).
+
+(* TODO: move *)
+Lemma ppo_helper : Cppo ⊆
+ ⦗CR⦘ ⨾ (certG.(data) ∪ certG.(ctrl) ∪ certG.(addr) ⨾ Csb^? ∪ Crfi ∪ Crmw ∪ certG.(rmw_dep) ⨾ Csb^?)^+ ⨾  
+   (⦗(R_ex certG.(lab)) \₁ dom_rel Crmw⦘ ⨾ Csb)^?⨾ ⦗CW⦘.
+Proof.
+Admitted.
+
+Lemma Cppo_in_Gar_int_ct : Cppo ;; <| dom_rel (Gar_int^+ ;; <| I |>) |> ⊆ Gar_int^+.
+Proof.
+unfold ppo.
+Admitted.
+
+Lemma Cppo_in_Gar_int_ct : Cppo ;; <| dom_rel (Car_int^+ ;; <| I |>) |> ⊆ Gar_int^+.
+Proof.
+unfold ppo.
+Admitted.
+
+Lemma Cppo_in_Gar_int_ct : Car_int^+ ;; <| I |> ⊆ Gar_int^+.
+Proof.
+unfold ppo.
+Admitted.
+
+
+Lemma cert_ppo_D : Cppo ⨾ ⦗ D ⦘ ⊆ Gppo.
+Proof using All.
+rewrite ppo_helper.
+unfold ppo; ins.
+
+rewrite cert_R, cert_W, cert_sb, cert_R_ex, !seqA.
+
+arewrite ((⦗GR_ex \₁ dom_rel Grmw⦘ ⨾ Gsb)^? ⨾ ⦗W⦘ ⨾ ⦗D⦘ ⊆ ⦗D⦘ ;; (⦗GR_ex \₁ dom_rel Grmw⦘ ⨾ Gsb)^? ⨾ ⦗W⦘).
+{ rewrite crE, !seq_union_l, !seqA.
+  forward (eapply dom_R_ex_fail_sb_D); try edone.
+  clear; basic_solver 12. }
+
+rewrite <- ct_cr with (r:=(Gdata ∪ Gctrl ∪ Gaddr ⨾ Gsb^? ∪ Grfi ∪ Grmw ∪ Grmw_dep ⨾ Gsb^? ∪ ⦗GR_ex \₁ dom_rel Grmw⦘ ⨾ Gsb)).
+hahn_frame_r.
+rewrite <- !seqA.
+apply seq_mori; [|clear; basic_solver 12].
+
+
+
+remember (Gdata ∪ Gctrl ∪ Gaddr ⨾ Gsb^? ∪ Grmw ∪ Grmw_dep ⨾ Gsb^?) as X.
+
+arewrite (Gdata ∪ Gctrl ∪ Gaddr ⨾ Gsb^? ∪ Crfi ∪ Grmw ∪ Grmw_dep ⨾ Gsb^? ⊆ X ∪ Crfi).
+{ subst X; clear; basic_solver 12. }
+
+assert (XX: X ∪ Grfi ⊆ Gdata ∪ Gctrl ∪ Gaddr ⨾ Gsb^? ∪ Grfi ∪ Grmw ∪ Grmw_dep ⨾ Gsb^? ∪ ⦗GR_ex \₁ dom_rel Grmw⦘ ⨾ Gsb).
+{ subst X; clear; basic_solver 12. }
+rewrite <- XX.
+(* arewrite (⦗W⦘ ⨾ ⦗D⦘ ⊆ ⦗D⦘ ⨾ ⦗W⦘) by basic_solver. *)
+(* hahn_frame. *)
+rewrite path_union; relsf; unionL.
+generalize inclusion_t_t; basic_solver.
+rewrite !seqA.
+
+assert (X_D_helper: dom_rel (X ⨾ ⦗D⦘) ⊆₁ D).
+{ rewrite HeqX.
+  relsf; unionL; splits.
+  eby eapply dom_data_D.
+  etransitivity; [|eby eapply dom_ctrl_in_D]; basic_solver.
+  etransitivity; [|eby eapply dom_addr_in_D]; basic_solver.
+  etransitivity; [|eby eapply dom_rmw_D]; basic_solver.
+  etransitivity; [|eby eapply dom_frmw_in_D]; basic_solver. }
+
+assert (X_D: dom_rel (X＊ ⨾ ⦗D⦘) ⊆₁ D).
+{ cut (X＊ ⨾ ⦗D⦘ ⊆ ⦗D⦘ ⨾ (fun _ _ => True)).
+by unfolder; ins; desf; eapply H; eauto.
+apply rt_ind_right with (P:= fun r =>  r ⨾ ⦗D⦘).
+- by eauto with hahn.
+- basic_solver.
+- intros h H; rewrite !seqA.
+rewrite (dom_rel_helper X_D_helper); sin_rewrite H.
+basic_solver. }
+
+
+rewrite (dom_rel_helper X_D).
+enough ((X＊ ⨾ Crfi)⁺ ⨾ ⦗D⦘ ⊆ (X ∪ Grfi)⁺).
+sin_rewrite H; arewrite (X ⊆ (X ∪ Grfi)⁺) at 2; relsf; basic_solver.
+
+
+apply ct_ind_right with (P:= fun r =>  r ⨾ ⦗D⦘).
+- by eauto with hahn.
+- rewrite !seqA, ct_end. 
+
+arewrite (X ⊆ X ∪ Grfi) at 1.
+rewrite cert_rfi_D.
+basic_solver 12.
+
+- intros k H.
+rewrite !seqA.
+rewrite cert_rfi_D.
+
+seq_rewrite (dom_rel_helper X_D).
+rewrite !seqA.
+sin_rewrite H.
+arewrite_id ⦗D⦘.
+arewrite (X ⊆ X ∪ Grfi) at 2.
+arewrite (Grfi ⊆ (X ∪ Grfi)＊) at 3.
+relsf.
+Qed.
+
+Lemma cert_ppo_CI : Cppo ⨾ ⦗ C ∪₁ I ⦘ ⊆ Gppo.
+Proof using All.
+rewrite C_in_D, I_in_D; relsf.
+apply cert_ppo_D.
+Qed.
+
+Lemma cert_detour_D : Cdetour ⨾ ⦗ D ⦘ ⊆ ⦗ I ⦘ ⨾ Gdetour.
+Proof using ACYC_EXT COH CSC Grfe_E IT_new_co RPPO_S ST_in_E S_in_W TCCOH WF WF_SC
+      detour_Acq_E detour_E.
+  enough (Cdetour ⨾ ⦗ D ⦘ ⊆ Gdetour).
+  { arewrite (⦗D⦘ ⊆ ⦗D⦘ ⨾ ⦗D⦘) by basic_solver.
+    sin_rewrite H.
+    forward (eapply dom_detour_D with (T:=T)); try edone.
+    clear. basic_solver. }
+  unfold detour, Execution.coe.
+  rewrite cert_sb.
+  rewrite <- seq_eqv_inter_lr, !seqA.
+  rewrite cert_rfe_D.
+  rewrite I_in_cert_co_base with (G:=G).
+  seq_rewrite <- seq_eqv_minus_lr.
+  ins; rewrite cert_co_I; try edone.
+  clear. basic_solver 21.
+Qed.
+
+Lemma cert_detour_R_Acq_sb_D : Cdetour ⨾ ⦗R∩₁Acq⦘ ⨾ Gsb ⨾ ⦗ D ⦘ ⊆ 
+  ⦗ I ⦘ ⨾ Gdetour ⨾ ⦗R∩₁Acq⦘ ⨾ Gsb.
+Proof using All.
+  rewrite (detour_to_codom_rfe WF_cert), !seqA.
+  rewrite cert_rfe.
+  rewrite codom_union, id_union; relsf; unionL.
+  arewrite (⦗codom_rel (⦗I⦘ ⨾ Grfe ⨾ ⦗D⦘)⦘ ⊆ ⦗D⦘) by basic_solver.
+  sin_rewrite cert_detour_D; basic_solver 40.
+  unfolder; ins; desf; exfalso.
+  generalize new_rfe_Acq. basic_solver 21.
+Qed.
+
+
+
+
+
+Lemma cert_ar_int_I : Car_int⁺ ⨾ ⦗ C ∪₁ I ⦘ ⊆ ⦗ D ∪₁ R ∩₁ Acq ⦘ ⨾ Gar_int⁺.
+Proof.
+
+rewrite (ct_ar_int_alt WF_cert).
+2: by apply (coherence_sc_per_loc cert_coherence).
+rewrite cert_R, cert_Acq, cert_sb, cert_W_ex_acq, cert_W.
+rewrite cert_same_loc, cert_Rel, cert_AcqRel, cert_F, cert_W_ex.
+  arewrite (⦗R ∩₁ Acq⦘ ⊆ ⦗Acq⦘ ;; ⦗R ∩₁ Acq⦘) at 3.
+  { clear; basic_solver. }
+  sin_rewrite Crfi_to_Acq_in_Grf.
+
+relsf; unionL.
+- unfold ar_int, bob, fwbob.
+case_refl Gsb.
+rewrite (dom_l (@wf_sbE G)) at 1.
+generalize E_F_AcqRel_in_C, C_in_D.
+rewrite <- ct_step; basic_solver 12.
+rewrite (dom_l (@wf_sbE G)) at 2.
+generalize E_F_AcqRel_in_C, (dom_sb_covered TCCOH), C_in_D.
+rewrite ct_begin, <- inclusion_t_rt, <- ct_step; basic_solver 32.
+- unfold ar_int, bob.
+rewrite <- ct_step; basic_solver 12.
+- unfold ar_int, bob, fwbob.
+case_refl Gsb.
+rewrite (dom_r (@wf_sbE G)) at 1.
+generalize E_F_AcqRel_in_C, (dom_sb_covered TCCOH), C_in_D.
+rewrite <- ct_step; basic_solver 21.
+rewrite (dom_r (@wf_sbE G)) at 1.
+generalize E_F_AcqRel_in_C, (dom_sb_covered TCCOH), C_in_D.
+rewrite ct_begin, <- inclusion_t_rt, <- ct_step; basic_solver 32.
+- unfold ar_int, bob, fwbob.
+rewrite W_rel_sb_loc_W_CI.
+generalize C_in_D, I_in_D.
+rewrite <- ct_step; basic_solver 21.
+- unfold ar_int, bob, fwbob.
+rewrite !seqA.
+rewrite (cr_helper W_rel_sb_loc_W_CI).
+rewrite <- seqA.
+sin_rewrite sb_W_rel_CI.
+generalize C_in_D, I_in_D.
+rewrite <- ct_cr, <- ct_step; basic_solver 32.
+
+- rewrite !seqA.
+rewrite (cr_helper W_rel_sb_loc_W_CI).
+
+arewrite ((⦗W ∩₁ Rel⦘ ⨾ Gsb ∩ Gsame_loc ⨾ ⦗W⦘)^?  ⊆ Gar_int^?) at 1.
+unfold ar_int, bob, fwbob; basic_solver 21.
+
+rewrite <- (ct_cr Gar_int).
+hahn_frame_r.
+
+arewrite (Cppo ⨾ ⦗C ∪₁ I⦘ ⊆ Gppo⨾ ⦗C ∪₁ I⦘).
+generalize cert_ppo_CI; basic_solver 12.
+
+arewrite (Gppo ⨾ ⦗C ∪₁ I⦘ ⊆ ⦗D⦘ ⨾ Gppo).
+rewrite C_in_D, I_in_D; generalize dom_ppo_D; basic_solver.
+
+
+rewrite <-ct_step.
+
+unfold ar_int; basic_solver 12.
+
+- rewrite !seqA.
+rewrite (cr_helper W_rel_sb_loc_W_CI).
+
+
+arewrite ((⦗W ∩₁ Rel⦘ ⨾ Gsb ∩ Gsame_loc ⨾ ⦗W⦘)^?  ⊆ Gar_int^?) at 3.
+unfold ar_int, bob, fwbob; basic_solver 21.
+
+rewrite <- (ct_cr Gar_int).
+hahn_frame_r.
+
+
+arewrite (Cppo^? ⨾ ⦗C ∪₁ I⦘ ⊆ Gppo^?⨾ ⦗C ∪₁ I⦘).
+generalize cert_ppo_CI; basic_solver 12.
+
+arewrite (Gppo^? ⨾ ⦗C ∪₁ I⦘ ⊆ ⦗D⦘ ⨾ Gppo^?).
+rewrite C_in_D, I_in_D; generalize dom_ppo_D; basic_solver.
+
+arewrite (Gppo^?  ⊆ Gar_int^?).
+unfold ar_int; basic_solver 12.
+
+rewrite <- (ct_cr Gar_int).
+hahn_frame_r.
+
+apply ct_inclusion_from_rt_inclusion1.
+
+{ rewrite detour_in_sb, !(ppo_in_sb WF_cert).
+arewrite_id ⦗W⦘ at 1.
+arewrite_id ⦗W⦘ at 1.
+arewrite_id ⦗R ∩₁ Acq⦘ at 1.
+arewrite_id  ⦗W ∩₁ Rel⦘ at 1.
+arewrite_id  ⦗W ∩₁ Rel⦘ at 1.
+arewrite_id  ⦗W ∩₁ Rel⦘ at 1.
+arewrite_id  ⦗GW_ex_acq⦘ at 1.
+arewrite (Gsb ∩ Gsame_loc ⊆ Gsb) at 1.
+arewrite_id  ⦗W ∩₁ Rel⦘ at 1.
+arewrite_id  ⦗GW_ex⦘ at 1.
+arewrite (Gsb ∩ Gsame_loc ⊆ Gsb) at 1.
+arewrite_id ⦗R ∩₁ Acq⦘ at 1.
+arewrite (Grfi ⊆ Gsb) at 1.
+
+rewrite cert_sb.
+arewrite_id  ⦗W ∩₁ Rel⦘ at 1.
+arewrite_id ⦗W⦘ at 1.
+generalize (@sb_trans G); ins; relsf.
+apply sb_acyclic. }
+
+
+
+apply rt_ind_right with (P:= fun r =>  r ⨾ ⦗D⦘).
+by auto with hahn.
+by basic_solver.
+
+intros k H; rewrite !seqA.
+
+ relsf; unionL.
+* case_refl (⦗R ∩₁ Acq⦘ ⨾ Gsb).
++
+rewrite cert_detour_D.
+
+arewrite (Gdetour  ⊆ Gar_int).
+rewrite (rt_end Gar_int); relsf; unionR right.
+hahn_frame_r.
+
+arewrite (⦗I⦘ ⊆ ⦗C ∪₁ I⦘).
+
+
+rewrite (cr_helper sb_W_rel_CI).
+
+arewrite ((Gsb ⨾ ⦗W ∩₁ Rel⦘)^?  ⊆ Gar_int^?).
+unfold ar_int, bob, fwbob; basic_solver 21.
+rewrite <- (rt_cr Gar_int).
+hahn_frame_r.
+
+arewrite (Cppo^? ⨾ ⦗C ∪₁ I⦘ ⊆ Gppo^? ⨾ ⦗C ∪₁ I⦘).
+generalize cert_ppo_CI; basic_solver 12.
+
+arewrite (Gppo^? ⨾ ⦗C ∪₁ I⦘ ⊆ ⦗D⦘ ⨾ Gppo^?  ).
+rewrite C_in_D, I_in_D; generalize dom_ppo_D; basic_solver.
+
+arewrite (Gppo ⊆ Gar_int).
+rewrite <- (rt_cr Gar_int).
+hahn_frame_r.
+
+done.
+
++
+rewrite !seqA, cert_detour_R_Acq_sb_D.
+arewrite (⦗R ∩₁ Acq⦘ ⨾ Gsb  ⊆ Gar_int).
+by unfold ar_int, bob, fwbob; basic_solver 21.
+
+rewrite (rt_end Gar_int); relsf; unionR right.
+hahn_frame_r.
+
+arewrite (Gdetour  ⊆ Gar_int^?).
+rewrite <- (rt_cr Gar_int).
+hahn_frame_r.
+arewrite (⦗I⦘ ⊆ ⦗C ∪₁ I⦘).
+rewrite (cr_helper sb_W_rel_CI).
+
+arewrite ((Gsb ⨾ ⦗W ∩₁ Rel⦘)^?  ⊆ Gar_int^?).
+unfold ar_int, bob, fwbob; basic_solver 21.
+rewrite <- (rt_cr Gar_int).
+hahn_frame_r.
+
+
+arewrite (Cppo^? ⨾ ⦗C ∪₁ I⦘ ⊆ Gppo^? ⨾ ⦗C ∪₁ I⦘).
+generalize cert_ppo_CI; basic_solver 12.
+
+arewrite (Gppo^? ⨾ ⦗C ∪₁ I⦘ ⊆ ⦗D⦘ ⨾ Gppo^?  ).
+rewrite C_in_D, I_in_D; generalize dom_ppo_D; basic_solver.
+
+arewrite (Gppo ⊆ Gar_int).
+rewrite <- (rt_cr Gar_int).
+hahn_frame_r.
+
+done.
+* 
+
+rewrite (dom_l (@wf_sbE G)) at 3; rewrite !seqA.
+
+arewrite (⦗GW_ex_acq⦘ ⨾ ⦗E⦘ ⊆ ⦗C ∪₁ I⦘ ⨾ ⦗GW_ex_acq⦘ ⨾ ⦗E⦘).
+generalize W_ex_acq_sb_S1; basic_solver 21.
+
+arewrite (⦗GW_ex_acq⦘ ⨾ ⦗E⦘ ⨾ Gsb ⨾ ⦗W⦘  ⊆ Gar_int^?).
+by unfold ar_int, bob, fwbob; basic_solver 21.
+arewrite_id ⦗D⦘; rels.
+rewrite <- (rt_cr Gar_int).
+hahn_frame_r.
+rewrite (cr_helper W_rel_sb_loc_W_CI).
+
+arewrite ((⦗W ∩₁ Rel⦘ ⨾ Gsb ∩ Gsame_loc ⨾ ⦗W⦘)^?  ⊆ Gar_int^?) at 1.
+unfold ar_int, bob, fwbob; basic_solver 21.
+
+rewrite <- (rt_cr Gar_int).
+hahn_frame_r.
+
+rewrite (cr_helper sb_W_rel_CI).
+
+arewrite ((Gsb ⨾ ⦗W ∩₁ Rel⦘)^?  ⊆ Gar_int^?).
+unfold ar_int, bob, fwbob; basic_solver 21.
+rewrite <- (rt_cr Gar_int).
+hahn_frame_r.
+
+arewrite (Cppo^? ⨾ ⦗C ∪₁ I⦘ ⊆ Gppo^? ⨾ ⦗C ∪₁ I⦘).
+generalize cert_ppo_CI; basic_solver 12.
+
+arewrite (Gppo^? ⨾ ⦗C ∪₁ I⦘ ⊆ ⦗D⦘ ⨾ Gppo^?  ).
+rewrite C_in_D, I_in_D; generalize dom_ppo_D; basic_solver.
+
+arewrite (Gppo ⊆ Gar_int).
+rewrite <- (rt_cr Gar_int).
+hahn_frame_r.
+
+done.
+
+*
+SearchAbout Grf Acq.
+Print ar_int.
+Print D.
+SearchAbout sb D.
+rewrite (dom_l WF.(wf_rfiE)).
+
+rewrite !seqA.
+
+arewrite (⦗GW_ex⦘ ⨾ ⦗E⦘ ⊆ ⦗C ∪₁ I⦘ ⨾ ⦗GW_ex⦘).
+generalize W_ex_E; basic_solver 21.
+
+arewrite (⦗GW_ex⦘ ⊆ ⦗GW_ex⦘ ;; ⦗set_compl Init⦘).
+by generalize (W_ex_not_init WF); basic_solver.
+sin_rewrite cert_rfi_Acq.
+rewrite !seqA.
+
+arewrite (⦗R ∩₁ Acq⦘ ⊆ ⦗R ∩₁ Acq⦘ ;; ⦗R ∩₁ Acq⦘).
+basic_solver.
+arewrite (⦗R ∩₁ Acq⦘ ⨾ Gsb^? ⊆ Gar_int^?).
+unfold ar_int, bob, fwbob; basic_solver 21.
+arewrite (⦗GW_ex⦘ ⨾ Grfi ⨾ ⦗R ∩₁ Acq⦘ ⊆ Gar_int^* ).
+rels.
+
+arewrite_id ⦗D⦘; rels.
+rewrite <- (rt_rt Gar_int) at 2.
+hahn_frame_r.
+rewrite (cr_helper W_rel_sb_loc_W_CI).
+
+arewrite ((⦗W ∩₁ Rel⦘ ⨾ Gsb ∩ Gsame_loc ⨾ ⦗W⦘)^?  ⊆ Gar_int^?) at 1.
+unfold ar_int, bob, fwbob; basic_solver 21.
+
+rewrite <- (rt_cr Gar_int).
+hahn_frame_r.
+
+rewrite (cr_helper sb_W_rel_CI).
+
+arewrite ((Gsb ⨾ ⦗W ∩₁ Rel⦘)^?  ⊆ Gar_int^?).
+unfold ar_int, bob, fwbob; basic_solver 21.
+rewrite <- (rt_cr Gar_int).
+hahn_frame_r.
+
+arewrite (Cppo^? ⨾ ⦗C ∪₁ I⦘ ⊆ Gppo^? ⨾ ⦗C ∪₁ I⦘).
+generalize cert_ppo_CI; basic_solver 12.
+
+arewrite (Gppo^? ⨾ ⦗C ∪₁ I⦘ ⊆ ⦗D⦘ ⨾ Gppo^?  ).
+rewrite C_in_D, I_in_D; generalize dom_ppo_D; basic_solver.
+
+arewrite (Gppo ⊆ Gar_int).
+rewrite <- (rt_cr Gar_int).
+hahn_frame_r.
+
+done.
+Qed.
+
+*)
+
+(*
+Lemma cert_ar_int_I : Car_int⁺ ⨾ ⦗ C ∪₁ I ⦘ ⊆ ⦗ D ∪₁ R ∩₁ Acq ⦘ ⨾ Gar_int⁺.
+Proof using All.
+  rewrite (ct_ar_int_alt WF_cert).
+  2: by apply (coherence_sc_per_loc cert_coherence).
+  rewrite cert_R, cert_Acq, cert_sb, cert_W_ex_acq, cert_W.
+  rewrite cert_same_loc, cert_Rel, cert_AcqRel, cert_F, cert_W_ex.
+  arewrite (⦗R ∩₁ Acq⦘ ⊆ ⦗Acq⦘ ;; ⦗R ∩₁ Acq⦘) at 3.
+  { clear; basic_solver. }
+  sin_rewrite Crfi_to_Acq_in_Grf.
+
+  relsf; unionL.
+  { unfold ar_int, bob, fwbob.
+    case_refl Gsb.
+    { rewrite (dom_l (@wf_sbE G)) at 1.
+      generalize E_F_AcqRel_in_C, C_in_D.
+      rewrite <- ct_step. basic_solver 12. }
+    rewrite (dom_l (@wf_sbE G)) at 2.
+    generalize E_F_AcqRel_in_C, (dom_sb_covered TCCOH), C_in_D.
+    rewrite ct_begin, <- inclusion_t_rt, <- ct_step.
+    basic_solver 32. }
+  { unfold ar_int, bob.
+    rewrite <- ct_step. basic_solver 12. }
+  { unfold ar_int, bob, fwbob.
+    case_refl Gsb.
+    { rewrite (dom_r (@wf_sbE G)) at 1.
+      generalize E_F_AcqRel_in_C, (dom_sb_covered TCCOH), C_in_D.
+      rewrite <- ct_step. basic_solver 21. }
+    rewrite (dom_r (@wf_sbE G)) at 1.
+    generalize E_F_AcqRel_in_C, (dom_sb_covered TCCOH), C_in_D.
+    rewrite ct_begin, <- inclusion_t_rt, <- ct_step.
+    basic_solver 32. }
+  { unfold ar_int, bob, fwbob.
+    rewrite W_rel_sb_loc_W_CI.
+    generalize C_in_D, I_in_D.
+    rewrite <- ct_step.
+    basic_solver 21. }
+  { unfold ar_int, bob, fwbob.
+    rewrite !seqA.
+    rewrite (cr_helper W_rel_sb_loc_W_CI).
+    rewrite <- seqA.
+    sin_rewrite sb_W_rel_CI.
+    generalize C_in_D, I_in_D.
+    rewrite <- ct_cr, <- ct_step.
+    basic_solver 32. }
+  { rewrite !seqA.
+    rewrite (cr_helper W_rel_sb_loc_W_CI).
+
+    arewrite ((⦗W ∩₁ Rel⦘ ⨾ Gsb ∩ Gsame_loc ⨾ ⦗W⦘)^?  ⊆ Gar_int^?) at 1.
+    { unfold ar_int, bob, fwbob. basic_solver 21. }
+    rewrite <- (ct_cr Gar_int).
+    hahn_frame_r.
+    arewrite (Cppo ⨾ ⦗C ∪₁ I⦘ ⊆ Gppo⨾ ⦗C ∪₁ I⦘).
+    { generalize cert_ppo_CI; basic_solver 12. }
+    arewrite (Gppo ⨾ ⦗C ∪₁ I⦘ ⊆ ⦗D⦘ ⨾ Gppo).
+    { rewrite C_in_D, I_in_D; generalize dom_ppo_D; basic_solver. }
+    rewrite <- ct_step.
+    unfold ar_int. basic_solver 12. }
+  rewrite !seqA.
+  rewrite (cr_helper W_rel_sb_loc_W_CI).
+  arewrite ((⦗W ∩₁ Rel⦘ ⨾ Gsb ∩ Gsame_loc ⨾ ⦗W⦘)^?  ⊆ Gar_int^?) at 2.
+  { unfold ar_int, bob, fwbob. basic_solver 21. }
+  
+  SearchAbout 
+  arewrite (⦗GW_ex⦘ ⨾ Grfi ⨾ ⦗R ∩₁ Acq⦘ ⨾ Gsb^?  ⊆ Gar_int^?) at 2.
+  { unfold ar_int, bob, fwbob. basic_solver 21. }
+
+  
+  
+  
+  rewrite <- (ct_cr Gar_int).
+  hahn_frame_r.
+  arewrite (Cppo^? ⨾ ⦗C ∪₁ I⦘ ⊆ Gppo^?⨾ ⦗C ∪₁ I⦘).
+  { generalize cert_ppo_CI. basic_solver 12. }
+  arewrite (Gppo^? ⨾ ⦗C ∪₁ I⦘ ⊆ ⦗D⦘ ⨾ Gppo^?).
+  { rewrite C_in_D, I_in_D. generalize dom_ppo_D. basic_solver. }
+  arewrite (Gppo^? ⊆ Gar_int^?).
+  rewrite <- (ct_cr Gar_int).
+  hahn_frame_r.
+  apply ct_inclusion_from_rt_inclusion1.
+  { rewrite detour_in_sb, !(ppo_in_sb WF_cert).
+    arewrite_id ⦗W⦘ at 1.
+    arewrite_id ⦗W⦘ at 1.
+    arewrite_id ⦗R ∩₁ Acq⦘ at 1.
+    arewrite_id  ⦗W ∩₁ Rel⦘ at 1.
+    arewrite_id  ⦗W ∩₁ Rel⦘ at 1.
+    arewrite_id  ⦗W ∩₁ Rel⦘ at 1.
+    arewrite_id  ⦗GW_ex_acq⦘ at 1.
+    arewrite (Gsb ∩ Gsame_loc ⊆ Gsb) at 1.
+    rewrite cert_sb.
+    generalize (@sb_trans G); ins; relsf.
+    apply sb_acyclic. }
+
+  apply rt_ind_right with (P:= fun r =>  r ⨾ ⦗D⦘).
+  { auto with hahn. }
+  { basic_solver. }
+  intros k H; rewrite !seqA.
+  relsf; unionL.
+  { case_refl (⦗R ∩₁ Acq⦘ ⨾ Gsb).
+    { rewrite cert_detour_D.
+      arewrite (Gdetour  ⊆ Gar_int).
+      rewrite (rt_end Gar_int); relsf; unionR right.
+      hahn_frame_r.
+      arewrite (⦗I⦘ ⊆ ⦗C ∪₁ I⦘).
+      rewrite (cr_helper sb_W_rel_CI).
+      arewrite ((Gsb ⨾ ⦗W ∩₁ Rel⦘)^?  ⊆ Gar_int^?).
+      { unfold ar_int, bob, fwbob. basic_solver 21. }
+      rewrite <- (rt_cr Gar_int).
+      hahn_frame_r.
+      arewrite (Cppo^? ⨾ ⦗C ∪₁ I⦘ ⊆ Gppo^? ⨾ ⦗C ∪₁ I⦘).
+      { generalize cert_ppo_CI. basic_solver 12. }
+      arewrite (Gppo^? ⨾ ⦗C ∪₁ I⦘ ⊆ ⦗D⦘ ⨾ Gppo^?  ).
+      { rewrite C_in_D, I_in_D. generalize dom_ppo_D. basic_solver. }
+      arewrite (Gppo ⊆ Gar_int).
+      rewrite <- (rt_cr Gar_int). by hahn_frame_r. }
+    rewrite !seqA, cert_detour_R_Acq_sb_D.
+    arewrite (⦗R ∩₁ Acq⦘ ⨾ Gsb  ⊆ Gar_int).
+    rewrite (rt_end Gar_int); relsf; unionR right.
+    hahn_frame_r.
+    arewrite (Gdetour  ⊆ Gar_int^?).
+    rewrite <- (rt_cr Gar_int).
+    hahn_frame_r.
+    arewrite (⦗I⦘ ⊆ ⦗C ∪₁ I⦘).
+    rewrite (cr_helper sb_W_rel_CI).
+    arewrite ((Gsb ⨾ ⦗W ∩₁ Rel⦘)^?  ⊆ Gar_int^?).
+    { unfold ar_int, bob, fwbob. basic_solver 21. }
+    rewrite <- (rt_cr Gar_int).
+    hahn_frame_r.
+    arewrite (Cppo^? ⨾ ⦗C ∪₁ I⦘ ⊆ Gppo^? ⨾ ⦗C ∪₁ I⦘).
+    { generalize cert_ppo_CI. basic_solver 12. }
+    arewrite (Gppo^? ⨾ ⦗C ∪₁ I⦘ ⊆ ⦗D⦘ ⨾ Gppo^?).
+    { rewrite C_in_D, I_in_D. generalize dom_ppo_D. basic_solver. }
+    arewrite (Gppo ⊆ Gar_int).
+    rewrite <- (rt_cr Gar_int). by hahn_frame_r. }
+  rewrite !seqA.
+  rewrite (dom_rel_helper dom_W_ex_acq_sb_W_D_in_CI).
+  rewrite (dom_l (@wf_sbE G)) at 3; rewrite !seqA.
+
+  arewrite (⦗GW_ex_acq⦘ ⨾ ⦗E⦘ ⨾ Gsb ⨾ ⦗W⦘  ⊆ Gar_int^?).
+  arewrite_id ⦗D⦘; rels.
+  rewrite <- (rt_cr Gar_int).
+  hahn_frame_r.
+  rewrite (cr_helper W_rel_sb_loc_W_CI).
+
+  arewrite ((⦗W ∩₁ Rel⦘ ⨾ Gsb ∩ Gsame_loc ⨾ ⦗W⦘)^?  ⊆ Gar_int^?) at 1.
+  unfold ar_int, bob, fwbob; basic_solver 21.
+
+  rewrite <- (rt_cr Gar_int).
+  hahn_frame_r.
+
+  rewrite (cr_helper sb_W_rel_CI).
+
+  arewrite ((Gsb ⨾ ⦗W ∩₁ Rel⦘)^?  ⊆ Gar_int^?).
+  unfold ar_int, bob, fwbob; basic_solver 21.
+  rewrite <- (rt_cr Gar_int).
+  hahn_frame_r.
+
+  arewrite (Cppo^? ⨾ ⦗C ∪₁ I⦘ ⊆ Gppo^? ⨾ ⦗C ∪₁ I⦘).
+  generalize cert_ppo_CI; basic_solver 12.
+
+  arewrite (Gppo^? ⨾ ⦗C ∪₁ I⦘ ⊆ ⦗D⦘ ⨾ Gppo^?  ).
+  rewrite C_in_D, I_in_D; generalize dom_ppo_D; basic_solver.
+
+  arewrite (Gppo ⊆ Gar_int).
+  rewrite <- (rt_cr Gar_int).
+  hahn_frame_r.
+
+  done.
+Qed.
+*)
+
+Lemma cert_acyc_ext : acyc_ext certG sc.
+Proof using All.
+red; unfold imm_s.ar.
+rewrite unionC.
+apply acyclic_union1.
+- rewrite (ar_int_in_sb WF_cert); apply sb_acyclic.
+- red; rewrite sc_rfe_ct_in_sc_rfe; unionL.
+  apply WF_SC.
+  arewrite (certG.(rfe) ⊆ certG.(rf)).
+  apply rf_irr, WF_cert.
+- rewrite sc_rfe_ct_in_sc_rfe.
+  arewrite ((sc ∪ rfe certG) ⊆ ⦗ C ∪₁ I ⦘ ⨾ (sc ∪ rfe certG)).
+  { unionL.
+    - rewrite (dom_l (wf_scD WF_SC)) at 1.
+      rewrite (dom_l (wf_scE WF_SC)) at 1.
+      arewrite (Sc ⊆₁ Acq/Rel) by mode_solver.
+      generalize E_F_AcqRel_in_C; basic_solver 12.
+      - rewrite cert_rfe; basic_solver 12. }
+Print ar_int.
+sin_rewrite cert_ar_int_I.
+
+rotate 1.
+rewrite <- seqA.
+rewrite (seq_union_l).
+arewrite_id  ⦗D ∪₁ R ∩₁ Acq⦘ at 1; rels.
+
+arewrite (rfe certG ⨾ ⦗D ∪₁ R ∩₁ Acq⦘ ⊆ Grfe).
+{ rewrite cert_rfe; relsf; unionL; [basic_solver 12|].
+
+rewrite wf_new_rfE.
+generalize new_rfe_Acq.
+unfolder; ins; desf; exfalso; basic_solver 21. }
+
+arewrite (sc ⊆ Gar＊).
+arewrite (Grfe ⊆ Gar＊).
+arewrite (Gar_int ⊆ Gar).
+relsf.
+red; relsf.
+Qed.
+
+
+(******************************************************************************)
+(** **   *)
+(******************************************************************************)
+
+(* TODO: move to another file , CertExcutionInit ?*)
+Lemma cert_imm_consistent : imm_consistent certG sc.
+Proof using All.
+red; splits; eauto using WF_SC_cert, cert_acyc_ext, cert_coh_sc, cert_complete, cert_coherence, cert_rmw_atomicity.
+Qed.
+
+End CertExec.
