src/simulation/Cert_hb.v
@@ -1,0 +1,555 @@
+From hahn Require Import Hahn.
+
+From imm Require Import Events.
+From imm Require Import Execution.
+From imm Require Import Execution_eco.
+From imm Require Import imm_bob imm_s_ppo.
+From imm Require Import imm_s_hb.
+From imm Require Import imm_s.
+From imm Require Import imm_common_more.
+From imm Require Import CertCOhelper.
+From imm Require Import CombRelations.
+
+Require Import AuxRel2.
+Require Import TraversalConfig.
+Require Import TraversalConfigAlt.
+Require Import TraversalConfigAltOld.
+Require Import ExtTraversalConfig.
+
+Require Import ImmProperties.
+
+Require Import Cert_co.
+Require Import Cert_D.
+Require Import Cert_rf.
+Require Import CertExecution2.
+
+Set Implicit Arguments.
+Remove Hints plus_n_O.
+
+Notation "'Tid_' t" := (fun x => tid x = t) (at level 1).
+Notation "'NTid_' t" := (fun x => tid x <> t) (at level 1).
+
+Section CertExec_hb.
+
+Variable G : execution.
+Variable sc : relation actid.
+
+Notation "'Init'" := (fun a => is_true (is_init a)).
+
+Notation "'E'" := G.(acts_set).
+Notation "'Gacts'" := G.(acts).
+Notation "'Glab'" := G.(lab).
+Notation "'Gsb'" := G.(sb).
+Notation "'Grf'" := G.(rf).
+Notation "'Gco'" := G.(co).
+Notation "'Grmw'" := G.(rmw).
+Notation "'Gdata'" := G.(data).
+Notation "'Gaddr'" := G.(addr).
+Notation "'Gctrl'" := G.(ctrl).
+Notation "'Gdeps'" := G.(deps).
+Notation "'Grmw_dep'" := G.(rmw_dep).
+
+Notation "'Gfre'" := G.(fre).
+Notation "'Grfe'" := G.(rfe).
+Notation "'Gcoe'" := G.(coe).
+Notation "'Grfi'" := G.(rfi).
+Notation "'Gfri'" := G.(fri).
+Notation "'Gcoi'" := G.(coi).
+Notation "'Gfr'" := G.(fr).
+Notation "'Geco'" := G.(eco).
+Notation "'Gdetour'" := G.(detour).
+Notation "'Gsw'" := G.(sw).
+Notation "'Grelease'" := G.(release).
+Notation "'Grs'" := G.(rs).
+Notation "'Ghb'" := G.(hb).
+Notation "'Gppo'" := G.(ppo).
+Notation "'Grppo'" := G.(rppo).
+Notation "'Gbob'" := G.(bob).
+Notation "'Gfwbob'" := G.(fwbob).
+Notation "'Gar'" := (G.(ar) sc).
+Notation "'Gar_int'" := (G.(ar_int)).
+Notation "'Gurr'" := (G.(urr) sc).
+Notation "'Gfurr'" := (G.(furr) sc).
+Notation "'Gmsg_rel'" := (G.(msg_rel) sc).
+
+Notation "'Gloc'" := (loc Glab).
+Notation "'Gval'" := (val Glab).
+Notation "'Gsame_loc'" := (same_loc Glab).
+
+Notation "'R'" := (fun a => is_true (is_r Glab a)).
+Notation "'W'" := (fun a => is_true (is_w Glab a)).
+Notation "'F'" := (fun a => is_true (is_f Glab a)).
+Notation "'GR_ex'" := (fun a => is_true (R_ex Glab a)).
+Notation "'GW_ex'" := G.(W_ex).
+Notation "'GW_ex_acq'" := (GW_ex ∩₁ (fun a => is_true (is_xacq Glab a))).
+
+Notation "'Loc_' l" := (fun x => Gloc x = Some l) (at level 1).
+Notation "'W_' l" := (W ∩₁ Loc_ l) (at level 1).
+Notation "'R_' l" := (R ∩₁ Loc_ l) (at level 1).
+
+Notation "'Pln'" := (fun a => is_true (is_only_pln Glab a)).
+Notation "'Rlx'" := (fun a => is_true (is_rlx Glab a)).
+Notation "'Rel'" := (fun a => is_true (is_rel Glab a)).
+Notation "'Acq'" := (fun a => is_true (is_acq Glab a)).
+Notation "'Acqrel'" := (fun a => is_true (is_acqrel Glab a)).
+Notation "'Acq/Rel'" := (fun a => is_true (is_ra Glab a)).
+Notation "'Sc'" := (fun a => is_true (is_sc Glab a)).
+Notation "'xacq'" := (fun a => is_true (is_xacq Glab a)).
+
+
+Variable T : trav_config.
+Variable S : actid -> Prop.
+
+Notation "'I'" := (issued T).
+Notation "'C'" := (covered T).
+
+Variable thread : BinNums.positive.
+
+Notation "'cert_co'" := (cert_co G T thread).
+
+Notation "'D'" := (D G T S thread).
+
+Notation "'new_rf'" := (new_rf G sc T S thread).
+Notation "'cert_rf'" := (cert_rf G sc T S thread).
+Notation "'cert_rfi'" := (cert_rfi G sc T S thread).
+Notation "'cert_rfe'" := (cert_rfe G sc T S thread).
+
+Hypothesis WF : Wf G.
+Hypothesis WF_SC : wf_sc G sc.
+Hypothesis RELCOV : W ∩₁ Rel ∩₁ I ⊆₁ C.
+Hypothesis TCCOH : tc_coherent G sc T.
+Hypothesis ACYC_EXT : acyc_ext G sc.
+Hypothesis CSC : coh_sc G sc.
+Hypothesis COH : coherence G.
+Hypothesis AT : rmw_atomicity G.
+
+Hypothesis IT_new_co: I ∪₁ E ∩₁ W ∩₁ Tid_ thread ≡₁ E ∩₁ W.
+Hypothesis E_to_S: E ⊆₁ C ∪₁ dom_rel (Gsb^? ⨾ ⦗S⦘).
+Hypothesis Grfe_E : dom_rel Grfe ⊆₁ I.
+Hypothesis E_F_AcqRel_in_C: E ∩₁ F ∩₁ Acq/Rel ⊆₁ C.
+Hypothesis COMP_ACQ: forall r (IN: (E ∩₁ R ∩₁ Acq) r), exists w, Grf w r.
+Hypothesis urr_helper: dom_rel ((Ghb ⨾ ⦗F ∩₁ Sc⦘)^? ⨾ sc^? ⨾ Ghb^? ⨾ Grelease ⨾ ⦗I⦘) ⊆₁ C.
+Hypothesis urr_helper_C: dom_rel ((Ghb ⨾ ⦗F ∩₁ Sc⦘)^? ⨾ sc^? ⨾ Ghb^? ⨾ (Grelease ⨾ Grf)^? ⨾ ⦗C⦘) ⊆₁ C.
+Hypothesis W_hb_sc_hb_to_I_NTid: dom_rel (⦗W⦘ ⨾ Ghb ⨾ (sc ⨾ Ghb)^? ⨾ ⦗I ∩₁ NTid_ thread⦘) ⊆₁ I.
+Hypothesis detour_E : dom_rel (Gdetour ⨾ ⦗E ∩₁ NTid_ thread⦘) ⊆₁ I.
+Hypothesis detour_Acq_E : dom_rel (Gdetour ⨾ ⦗E ∩₁ R ∩₁ Acq⦘) ⊆₁ I.
+Hypothesis hb_sc_hb_de : ⦗(E \₁ C) ∩₁ (E \₁ I)⦘ ⨾ Ghb ⨾ (sc ⨾ Ghb)^? ⊆ Gsb.
+Hypothesis COMP_C : C ∩₁ R ⊆₁ codom_rel Grf.
+Hypothesis COMP_NTID : E ∩₁ NTid_ thread ∩₁ R ⊆₁ codom_rel Grf.
+Hypothesis COMP_PPO : dom_rel (Gppo ⨾ ⦗I⦘) ⊆₁ codom_rel Grf.
+Hypothesis COMP_RPPO : dom_rel (⦗R⦘ ⨾ (Gdata ∪ Grfi ∪ Grmw)＊ ⨾ Grppo ⨾ ⦗S⦘) ⊆₁ codom_rel Grf.
+Hypothesis TCCOH_rst_new_T : tc_coherent G sc (mkTC (C ∪₁ (E ∩₁ NTid_ thread)) I).
+
+Hypothesis S_in_W : S ⊆₁ W.
+Hypothesis RPPO_S : dom_rel ((Gdetour ∪ Grfe) ⨾ (Gdata ∪ Grfi ∪ Grmw)＊ ⨾ Grppo ⨾ ⦗S⦘) ⊆₁ I.
+Hypothesis ST_in_E : S ∩₁ Tid_ thread ⊆₁ E.
+Hypothesis I_in_S : I ⊆₁ S.
+Hypothesis W_ex_acq_in_I :GW_ex_acq ⊆₁ I.
+
+Hypothesis F_in_C : E ∩₁ F ∩₁ Acq/Rel ⊆₁ C.
+
+Hypothesis S_I_in_W_ex : (S ∩₁ Tid_ thread) \₁ I ⊆₁ W_ex G.
+
+Hypothesis ETC_DR_R_ACQ_I : dom_rel ((Gdetour ∪ Grfe) ⨾ (Grmw ⨾ Grfi)^* ⨾ ⦗R∩₁Acq⦘ ⨾ Gsb ⨾ ⦗S⦘) ⊆₁ I.
+
+Hypothesis COMP_R_ACQ_SB : dom_rel ((Grmw ⨾ Grfi)＊ ⨾ ⦗E ∩₁ R ∩₁ Acq⦘) ⊆₁ codom_rel Grf.
+
+Variable lab' : actid -> label.
+Hypothesis SAME : same_lab_u2v lab' Glab.
+
+Notation "'certG'" := (certG G sc T S thread lab').
+
+
+(* Notation "'CE'" := certG.(acts_set). *)
+(* Notation "'Cacts'" := certG.(acts). *)
+(* Notation "'Clab'" := certG.(lab). *)
+(* Notation "'Csb'" := certG.(sb). *)
+Notation "'Crf'" := certG.(rf).
+Notation "'Cco'" := certG.(co).
+Notation "'Crmw'" := certG.(rmw).
+(* Notation "'Cdata'" := certG.(data). *)
+(* Notation "'Caddr'" := certG.(addr). *)
+(* Notation "'Cctrl'" := certG.(ctrl). *)
+Notation "'Cdeps'" := certG.(deps).
+(* Notation "'Crmw_dep'" := certG.(rmw_dep). *)
+
+Notation "'Cfre'" := certG.(fre).
+(* Notation "'Crfe'" := certG.(rfe). *)
+Notation "'Ccoe'" := certG.(coe).
+Notation "'Crfi'" := certG.(rfi).
+Notation "'Cfri'" := certG.(fri).
+Notation "'Ccoi'" := certG.(coi).
+Notation "'Cfr'" := certG.(fr).
+Notation "'Ceco'" := certG.(eco).
+Notation "'Cdetour'" := certG.(detour).
+Notation "'Csw'" := certG.(sw).
+Notation "'Crelease'" := certG.(release).
+Notation "'Crs'" := certG.(rs).
+Notation "'Chb'" := certG.(hb).
+Notation "'Cppo'" := certG.(ppo).
+(* Notation "'Cbob'" := certG.(bob). *)
+(* Notation "'Cfwbob'" := certG.(fwbob). *)
+Notation "'Car'" := (certG.(ar) sc).
+Notation "'Car_int'" := (certG.(ar_int)).
+Notation "'Curr'" := (certG.(urr) sc).
+Notation "'Cmsg_rel'" := (certG.(msg_rel) sc).
+
+(* Notation "'E'" := G.(acts_set). *)
+(* Notation "'Gacts'" := G.(acts). *)
+Notation "'Clab'" := certG.(lab).
+Notation "'Csb'" := certG.(sb).
+(* Notation "'Grf'" := G.(rf). *)
+(* Notation "'Gco'" := G.(co). *)
+(* Notation "'Gdata'" := G.(data). *)
+(* Notation "'Gaddr'" := G.(addr). *)
+(* Notation "'Gctrl'" := G.(ctrl). *)
+(* Notation "'Gdeps'" := G.(deps). *)
+(* Notation "'Grmw_dep'" := G.(rmw_dep). *)
+
+(* Notation "'Gfre'" := G.(fre). *)
+Notation "'Crfe'" := certG.(rfe).
+(* Notation "'Gcoe'" := G.(coe). *)
+Notation "'Crfi'" := certG.(rfi).
+(* Notation "'Gfri'" := G.(fri). *)
+(* Notation "'Gcoi'" := G.(coi). *)
+(* Notation "'Gfr'" := G.(fr). *)
+(* Notation "'Geco'" := G.(eco). *)
+(* Notation "'Gdetour'" := G.(detour). *)
+(* Notation "'Gsw'" := G.(sw). *)
+Notation "'Crelease'" := certG.(release).
+(* Notation "'Grs'" := G.(rs). *)
+(* Notation "'Ghb'" := G.(hb). *)
+(* Notation "'Gppo'" := G.(ppo). *)
+(* Notation "'Grppo'" := G.(rppo). *)
+(* Notation "'Gbob'" := G.(bob). *)
+(* Notation "'Gfwbob'" := G.(fwbob). *)
+(* Notation "'Gar'" := (G.(ar) sc). *)
+(* Notation "'Gar_int'" := (G.(ar_int)). *)
+(* Notation "'Gurr'" := (G.(urr) sc). *)
+(* Notation "'Gfurr'" := (G.(furr) sc). *)
+(* Notation "'Gmsg_rel'" := (G.(msg_rel) sc). *)
+
+(* Notation "'Gloc'" := (loc Glab). *)
+(* Notation "'Gval'" := (val Glab). *)
+Notation "'Csame_loc'" := (same_loc Clab).
+
+Notation "'CR'" := (fun a => is_true (is_r Clab a)).
+Notation "'CW'" := (fun a => is_true (is_w Clab a)).
+Notation "'CF'" := (fun a => is_true (is_f Clab a)).
+(* Notation "'GR_ex'" := (fun a => is_true (R_ex Glab a)). *)
+(* Notation "'GW_ex'" := G.(W_ex). *)
+(* Notation "'GW_ex_acq'" := (GW_ex ∩₁ (fun a => is_true (is_xacq Glab a))). *)
+
+Notation "'CPln'" := (fun a => is_true (is_only_pln Clab a)).
+Notation "'CRlx'" := (fun a => is_true (is_rlx Clab a)).
+Notation "'CRel'" := (fun a => is_true (is_rel Clab a)).
+Notation "'CAcq'" := (fun a => is_true (is_acq Clab a)).
+Notation "'CAcqrel'" := (fun a => is_true (is_acqrel Clab a)).
+Notation "'CAcq/Rel'" := (fun a => is_true (is_ra Clab a)).
+Notation "'CSc'" := (fun a => is_true (is_sc Clab a)).
+
+
+(******************************************************************************)
+(** **   *)
+(******************************************************************************)
+
+Lemma dom_rf_D_helper: Grf ⨾ ⦗D⦘ ≡ ⦗D⦘ ;; Grf ⨾ ⦗D⦘.
+Proof.
+forward (eapply dom_rf_D with (T:=T) (S:=S) (thread:=thread)); try edone.
+basic_solver 12.
+Qed.
+
+Lemma Grelease_D_in_Crelease : Grelease ;; <| D |> ⊆ Crelease.
+Proof using All.
+  unfold release, rs; ins.
+  rewrite (cert_F _ SAME).
+  rewrite (cert_Rel _ SAME).
+  rewrite (cert_W _ SAME).
+  rewrite (cert_same_loc _ SAME).
+  rewrite (cert_sb).
+  hahn_frame.
+  transitivity ((Grf ⨾ ⦗D⦘ ⨾ Grmw)＊).
+  2: unfold Cert_rf.cert_rf; apply clos_refl_trans_mori; basic_solver 12.
+  eapply rt_ind_right with (P:=fun r=> r ;; ⦗D⦘); eauto with hahn.
+  basic_solver 12.
+  intros k H.
+  rewrite !seqA.
+  arewrite (Grmw ⨾ ⦗D⦘ ⊆ ⦗D⦘ ;; Grmw) at 1.
+  { forward (eapply dom_rmw_D with (T:=T)); try edone; basic_solver. }
+  remember ((Grf ⨾ ⦗D⦘ ⨾ Grmw)＊) as X.
+  seq_rewrite dom_rf_D_helper.
+  subst X.
+  rewrite !seqA.
+  sin_rewrite H.
+  rewrite rtE at 2.
+  rewrite ct_end.
+  basic_solver 21.
+Qed.
+
+Lemma Crelease_D_in_Grelease : Crelease ;; <| D |> ⊆ Grelease.
+Proof using All.
+  unfold release, rs; ins.
+  rewrite (cert_F _ SAME).
+  rewrite (cert_Rel _ SAME).
+  rewrite (cert_W _ SAME).
+  rewrite (cert_same_loc _ SAME).
+  rewrite (cert_sb).
+  hahn_frame.
+  transitivity ((Grf ⨾ ⦗D⦘ ⨾ Grmw)＊).
+  2: apply clos_refl_trans_mori; basic_solver 12.
+  eapply rt_ind_right with (P:=fun r=> r ;; ⦗D⦘); eauto with hahn.
+  basic_solver 12.
+  intros k H.
+  rewrite !seqA.
+  arewrite (Grmw ⨾ ⦗D⦘ ⊆ ⦗D⦘ ;; Grmw) at 1.
+  { forward (eapply dom_rmw_D with (T:=T)); try edone; basic_solver. }
+  arewrite (cert_rf ⨾ ⦗D⦘ ⊆ Grf ⨾ ⦗D⦘) by (by apply cert_rf_D).
+  remember ((Grf ⨾ ⦗D⦘ ⨾ Grmw)＊) as X.
+  seq_rewrite dom_rf_D_helper.
+  subst X.
+  rewrite !seqA.
+  sin_rewrite H.
+  rewrite rtE at 2.
+  rewrite ct_end.
+  basic_solver 21.
+Qed.
+
+Lemma Crelease_D_eq_Grelease_D : Crelease ;; <| D |> ≡ Grelease ;; <| D |>.
+Proof using All.
+  generalize Crelease_D_in_Grelease, Grelease_D_in_Crelease.
+  clear. basic_solver.
+Qed.
+
+(*Lemma rt_rf_rmw : (rf ⨾ rmw)＊ ⊆ (rfi ⨾ rmw)＊ ⨾ (rfe ⨾ rmw ⨾ (rfi ⨾ rmw)＊)＊.
+Proof.
+eapply rt_ind_left with (P:=fun r=> r); eauto with hahn.
+basic_solver 12.
+intros k H.
+rewrite !seqA, H.
+rewrite rfi_union_rfe; relsf; unionL.
+- rewrite rt_begin at 3.
+  basic_solver 21.
+- rewrite (rt_begin (rfe ⨾ rmw ⨾ (rfi ⨾ rmw)＊)) at 2.
+  basic_solver 21.
+Qed.
+*)
+Lemma cert_sb_sw_helper : Gsb ∪ Gsw ⊆ Gsb ∪ Csw.
+Proof using All.
+  unionL; [basic_solver|].
+  unfold imm_s_hb.sw; ins.
+  remember (Grf ⨾ ⦗D⦘ ∪ new_rf) as X.
+  rewrite (cert_F _ SAME).
+  rewrite (cert_Acq _ SAME).
+  rewrite (cert_sb).
+  rewrite !crE, !seq_union_l, !seq_union_r, !seq_id_l, !seqA.
+  unionL.
+  { arewrite (⦗Acq⦘ ⊆ (⦗D⦘ ∪ ⦗set_compl D⦘) ⨾ ⦗Acq⦘) at 1.
+    { unfolder. ins. desf. destruct (classic (D y)); eauto. }
+    rewrite !seq_union_l, !seq_union_r.
+    unionL.
+    { seq_rewrite dom_rf_D_helper.
+      rewrite !seqA.
+      sin_rewrite Grelease_D_in_Crelease.
+      unfold Cert_rf.cert_rf.
+      subst X; basic_solver 21. }
+    rewrite rfi_union_rfe at 1.
+    rewrite !seq_union_l, !seq_union_r.
+    unionL; cycle 1.
+    { transitivity (fun _ _ : actid => False); [|basic_solver].
+      rewrite (dom_r WF.(wf_rfeD)).
+      unfold Cert_D.D; basic_solver 21. }
+    rewrite (dom_r WF.(wf_rfiE)) at 1.
+    rewrite E_to_S.
+    rewrite C_in_D with (G:=G) (T:=T) (S:=S) (thread:=thread). 
+    rewrite id_union, !seq_union_r, !seq_union_l, !seq_union_r, !seqA.
+    unionL; [basic_solver|].
+    unfold release at 1, rs at 1.
+    rewrite rt_rf_rmw.
+    rewrite rtE with (r:= Grfe ⨾ Grmw ⨾ (Grfi ⨾ Grmw)＊).
+    rewrite !seq_union_r, !seq_union_l; unionL.
+    { arewrite (Grfi ⊆ Gsb).
+      rewrite WF.(rmw_in_sb).
+      generalize (@sb_trans G); ins; relsf.
+      revert H; basic_solver 21. }
+    rewrite ct_end, <- !seqA.
+    arewrite (((((((⦗Rel⦘ ⨾ (⦗F⦘ ⨾ Gsb)^?) ⨾ ⦗W⦘) ⨾ (Gsb ∩ Gsame_loc)^?) ⨾ ⦗W⦘) ⨾ 
+      (Grfi ⨾ Grmw)＊) ⨾ ((Grfe ⨾ Grmw) ⨾ (Grfi ⨾ Grmw)＊)＊) ⊆ Grelease).
+    { arewrite (Grfi ⊆ Grf).
+      arewrite (Grfe ⊆ Grf).
+      rewrite <- !seqA.
+      rewrite <- !ct_begin.
+      rewrite !seqA; relsf. }
+    assert (BB: Grmw ⨾ (Grfi ⨾ Grmw)＊ ⨾ Grfi ⊆ (Grmw ⨾ Grfi)^+).
+    { seq_rewrite <- rt_seq_swap.
+      rewrite !seqA.
+      remember (Grmw ⨾ Grfi) as Y.
+      apply ct_end. }
+    sin_rewrite BB.
+    assert (AA: dom_rel (Grfe ⨾ (Grmw ⨾ Grfi)⁺ ⨾ ⦗dom_rel (Gsb^? ⨾ ⦗S⦘)⦘ ⨾ ⦗Acq⦘) ⊆₁ I).
+    { rewrite (dom_r WF.(wf_rfiD)) at 1.
+      rewrite seq_eqvC.
+      rewrite <- !seqA.
+      rewrite dom_rel_eqv_dom_rel, seqA. rewrite inclusion_ct_seq_eqv_r, !seqA.
+      arewrite (⦗R⦘ ⨾ ⦗Acq⦘ ⨾ Gsb^? ⨾ ⦗S⦘ ⊆ ⦗R ∩₁ Acq⦘ ⨾ Gsb ⨾ ⦗S⦘).
+      { rewrite crE; relsf. rewrite S_in_W at 1. type_solver 32. }
+      arewrite (Grfe ⊆ Gdetour ∪ Grfe). 
+      by rewrite inclusion_t_rt. }
+    rewrite seq_eqvC.
+    seq_rewrite (dom_rel_helper AA).
+    rewrite !seqA.
+    arewrite ((Grmw ⨾ Grfi)⁺ ⨾ ⦗dom_rel (Gsb^? ⨾ ⦗S⦘)⦘ ⨾ ⦗Acq⦘ ⊆ 
+              ⦗dom_rel ((Grmw ⨾ Grfi)＊ ⨾ ⦗R ∩₁ Acq⦘ ⨾ Gsb ⨾ ⦗S⦘)⦘ ⨾ 
+              (Grmw ⨾ Grfi)⁺ ⨾ ⦗dom_rel (Gsb^? ⨾ ⦗S⦘)⦘ ⨾ ⦗Acq⦘).
+    { apply dom_rel_helper.
+    rewrite seq_eqvC, <- seqA.
+    
+    rewrite dom_rel_eqv_dom_rel.
+    rewrite (dom_r WF.(wf_rfiD)) at 1. 
+    rewrite <- !seqA.
+    rewrite inclusion_ct_seq_eqv_r, !seqA.
+    arewrite (⦗S⦘ ⊆ ⦗S⦘ ;; ⦗W⦘) at 1.
+    { generalize S_in_W; clear; basic_solver. }
+    arewrite (⦗R⦘ ⨾ ⦗Acq⦘ ⨾ Gsb^? ⨾ ⦗S⦘ ;; ⦗W⦘ ⊆ ⦗R ∩₁ Acq⦘ ⨾ Gsb ⨾ ⦗S⦘).
+    {  type_solver 21. }
+    rewrite rtE. basic_solver 21. }
+    arewrite (Grfe ⊆ Grf).
+arewrite (Grf
+    ⨾ ⦗dom_rel ((Grmw ⨾ Grfi)＊ ⨾ ⦗R ∩₁ Acq⦘ ⨾ Gsb ⨾ ⦗S⦘)⦘  ⊆ Crf).
+apply Grf_to_Acq_S_in_cert_rf; edone.
+
+    rewrite Grfi_in_cert_rfi at 1; try edone.
+    arewrite_id ⦗dom_rel (Gsb^? ⨾ ⦗S⦘)⦘.
+    arewrite_id ⦗set_compl D⦘.
+    arewrite (Crfi ⊆ Crf).
+    seq_rewrite <- ct_seq_swap.
+    rewrite !seqA.
+    arewrite (Grelease ⨾ ⦗I⦘ ⊆ release certG).
+    { rewrite I_in_D; apply Grelease_D_in_Crelease. }
+  rels.
+  rewrite inclusion_t_rt.
+  rewrite <- cert_rmw.
+  sin_rewrite release_rf_rmw_steps.
+  subst X; ins; basic_solver 12. }
+  
+arewrite (⦗F⦘ ⨾ ⦗Acq⦘ ⊆ ⦗F ∩₁ Acq/Rel⦘ ⨾ ⦗Acq⦘) at 1.
+by mode_solver 21.
+
+arewrite (Gsb ⨾ ⦗F ∩₁ Acq/Rel⦘ ⊆ ⦗D⦘ ;; Gsb ⨾ ⦗F ∩₁ Acq/Rel⦘).
+{ forward (eapply dom_sb_F_AcqRel_in_D with (T:=T) (S:=S) (thread:=thread)); try edone.
+  basic_solver 12. }
+
+  seq_rewrite dom_rf_D_helper.
+  rewrite !seqA.
+
+arewrite ( Grf ⨾ ⦗D⦘ ⊆ cert_rf).
+
+sin_rewrite Grelease_D_in_Crelease.
+unionR right -> right.
+basic_solver 21.
+Qed.
+
+Lemma cert_sb_sw : Gsb ∪ Csw ≡ Gsb ∪ Gsw.
+Proof using All.
+  split; [|by apply cert_sb_sw_helper].
+  unionL; [by eauto with hahn|].
+  unfold imm_s_hb.sw; ins.
+  rewrite (cert_F _ SAME).
+  rewrite (cert_Acq _ SAME).
+  rewrite (cert_sb).
+  rewrite !crE, !seq_union_l, !seq_union_r, !seq_id_l.
+  unionL.
+  2: { rewrite !seqA.
+       arewrite (Gsb ⨾ ⦗F⦘ ⨾ ⦗Acq⦘ ≡ ⦗D⦘ ⨾ Gsb ⨾ ⦗F⦘ ⨾ ⦗Acq⦘).
+       { rewrite (dom_r (@wf_sbE G)). generalize dom_sb_F_Acq_in_D. basic_solver 12. }
+       arewrite (cert_rf ⨾ ⦗D⦘ ⊆ Grf ⨾ ⦗D⦘) by (by apply cert_rf_D).
+       seq_rewrite dom_rf_D_helper.
+       rewrite !seqA.
+       seq_rewrite Crelease_D_eq_Grelease_D.
+       rewrite !seqA. eauto with hahn. }
+  arewrite (cert_rf ⊆ cert_rf ;; <|D|> ∪ cert_rf ;; <|set_compl D|>).
+  { clear. unfolder. ins. desf. tauto. }
+  rewrite !seq_union_l, !seq_union_r.
+  unionL.
+  { arewrite (cert_rf ⨾ ⦗D⦘ ⊆ Grf ⨾ ⦗D⦘) by (by apply cert_rf_D).
+    seq_rewrite dom_rf_D_helper.
+    rewrite !seqA.
+    seq_rewrite Crelease_D_eq_Grelease_D.
+    basic_solver 20. }
+  rewrite cert_rfD; try edone.
+  rewrite cert_rfE; try edone.
+  rewrite !seqA.
+  rewrite <- !id_inter. rewrite <- set_interA.
+  arewrite (E ∩₁ R ∩₁ (set_compl D ∩₁ Acq) ⊆₁
+            codom_rel Grf ∩₁ set_compl D ∩₁ (E ∩₁ R ∩₁ Acq)).
+  { generalize COMP_ACQ. clear. basic_solver 10. }
+  rewrite rfi_union_rfe at 1. rewrite codom_union.
+  rewrite set_inter_union_l. rewrite set_inter_union_l, id_union, !seq_union_r.
+  unionL.
+  2: { arewrite (codom_rel Grfe ∩₁ set_compl D ∩₁ (E ∩₁ R ∩₁ Acq) ⊆₁ ∅).
+       { unfold Cert_D.D. basic_solver 20. }
+       basic_solver. }
+  rewrite !id_inter. rewrite !seqA.
+  arewrite (cert_rf ⨾ ⦗codom_rel Grfi⦘ ⨾ ⦗set_compl D⦘ ⊆ Grfi ⨾ ⦗set_compl D⦘).
+  { rewrite <- id_inter.
+    intros x y HH.
+    apply seq_eqv_r in HH. destruct HH as [HH [[x' AA] BB]].
+    assert (x' = x); subst; auto.
+    { eapply cert_rff; eauto.
+      apply Grfi_in_cert_rfi; auto. }
+    basic_solver. }
+  unfold release at 1, rs at 1.
+  rewrite rt_rf_rmw.
+  rewrite rtE with (r:= rfe certG ⨾ Crmw ⨾ (rfi certG ⨾ Crmw)＊).
+  rewrite !seq_union_r, !seq_union_l; unionL.
+  { unionR left.
+    arewrite (Crfi ⊆ Gsb). arewrite (Grfi ⊆ Gsb).
+    rewrite WF.(rmw_in_sb).
+    generalize (@sb_trans G); ins; relsf.
+    revert H; basic_solver 21. }
+  unionR right -> left.
+  rewrite ct_end, <- !seqA.
+  arewrite (((((((⦗CRel⦘ ⨾ (⦗CF⦘ ⨾ Csb)^?) ⨾ ⦗CW⦘) ⨾ (Csb ∩ Csame_loc)^?) ⨾ ⦗CW⦘) ⨾ 
+               (Crfi ⨾ Crmw)＊) ⨾ ((Crfe ⨾ Crmw) ⨾ (Crfi ⨾ Crmw)＊)＊) ⊆ Crelease).
+  { arewrite (Crfi ⊆ Crf).
+    arewrite (Crfe ⊆ Crf).
+    rewrite <- !seqA.
+    rewrite <- !ct_begin.
+    rewrite !seqA; relsf. }
+  arewrite (⦗set_compl D⦘ ⨾ ⦗E⦘ ⨾ ⦗R⦘ ⨾ ⦗Acq⦘ ⊆ ⦗Acq \₁ C⦘ ;; ⦗E ∩₁ R ∩₁ Acq \₁ C⦘).
+  { rewrite <- C_in_D. clear. basic_solver. }
+  rewrite cert_rmw.
+  arewrite_id (⦗W⦘ ⨾ ⦗E⦘). by basic_solver. 
+  rels.
+  arewrite ((Crfi ⨾ Grmw)＊ ⨾ Grfi ⨾ ⦗Acq \₁ C⦘  ⊆ (Grfi ⨾ Grmw)＊ ⨾ Grfi).
+  { rewrite cert_rfi_eq.
+    eapply cert_rfi_Grmw_rt_in_Grfi_Grmw; edone. }
+
+  arewrite (Crfe ⊆ <| I |> ;; Crfe).
+  { rewrite cert_rfe_eq.
+    eapply dom_rel_helper with (r:=cert_rfe).
+    eapply dom_cert_rfe_in_I; edone. }
+
+  rewrite I_in_D.
+  seq_rewrite Crelease_D_eq_Grelease_D.
+  rewrite !seqA.
+  arewrite (Crfe ⊆ Crf).
+  arewrite (Grmw ⨾ (Grfi ⨾ Grmw)＊ ⨾ Grfi ⊆ (Grmw ⨾ Grfi)＊).
+  { rewrite rt_seq_swap. rewrite <- seqA, <- ct_begin. apply inclusion_t_rt. }
+  rewrite r_to_dom_rel_r_r with (r:=(Grmw ⨾ Grfi)＊ ⨾ ⦗E ∩₁ R ∩₁ Acq \₁ C⦘).
+
+  arewrite (Crf ;; <| dom_rel ((Grmw ⨾ Grfi)^* ⨾ ⦗E∩₁R∩₁Acq \₁ C⦘) |> ⊆ Grf).
+  { rewrite cert_rf_eq.
+    eapply cert_rf_to_Acq_nC_in_Grf; edone. }
+
+  arewrite_id ⦗D⦘. rewrite seq_id_l.
+  arewrite (Grfi ⊆ Grf).
+  seq_rewrite <- rt_seq_swap. rewrite !seqA.
+  sin_rewrite release_rf_rmw_steps.
+  clear. basic_solver.
+Qed.
+
+Lemma cert_hb : Chb ≡ Ghb.
+Proof using All. by unfold imm_s_hb.hb; rewrite cert_sb_sw. Qed.
+
+
+End CertExec_hb.
